Imp/Stmt/Optimize.lean
@@ -6,27 +6,4 @@ namespace Imp.Stmt
 
 /-- Optimize a statement -/
 def optimize : Stmt → Stmt
-  | imp {skip;} => imp {skip;}
-  | imp {~s1 ~s2} =>
-    match s1.optimize, s2.optimize with
-    | imp {skip;}, s2' => s2'
-    | s1', imp {skip;} => s1'
-    | s1', s2' => imp {~s1' ~s2'}
-  | imp {if (~c) {~s1} else {~s2}} =>
-    let c' := c.optimize
-    match c' with
-    | .const 0 => s2.optimize
-    | .const _ => s1.optimize
-    | _ =>
-      let s1' := s1.optimize
-      let s2' := s2.optimize
-      if s1' = s2' then
-        s1'
-      else imp {if (~c') {~s1.optimize} else {~s2.optimize}}
-  | imp {while (~c) {~s}} =>
-    let c' := c.optimize
-    match c' with
-    | .const 0 => imp {skip;}
-    | _ => imp {while (~c') {~s.optimize}}
-  | imp {~x := ~e;} =>
-    imp {~x := ~e.optimize;}
+  | stmt => stmt
